README.md
@@ -1,5 +1,4 @@
-# AWS-Dafny
-Current Design of DateTime API
+# LocalDateTime
 
 Regarding the "absence of leap years every 4000 years," I checked how major programming languages determine leap years and found that none of them use the 4000-year rule. I think we can ignore this very rare rule.
 
@@ -7,8 +6,13 @@ The date calculation logic is now based on epoch time, so we have already avoide
 
 The new logic first converts the LocalDateTime to an epoch time in milliseconds. It also converts the time to be added or subtracted into milliseconds. Then, it performs the addition or subtraction. Finally, it converts the resulting millisecond time back to a LocalDateTime.
 
-## How to execute the test example
+## Execute Verification
 
+```
+dafny test --target:cs --standard-libraries LocalDateTime.dfy TestLocalDateTime.dfy  DateTimeImpl.cs --allow-warnings
+```
+
+## Run Test
 ```
 dafny build TestLocalDateTime.dfy --target:cs TestLocalDateTime.dfy DateTimeImpl.cs --standard-libraries
 
